Trident/Compiler.lean
@@ -6,7 +6,7 @@ namespace Trident
 def compiledVectorAdd : TritonKernel := [
   { result := "pid",    op := .get_program_id 0, args := [] },
   { result := "bstart", op := .muli,              args := ["pid", "bsize"] },
-  { result := "range",  op := .make_range,         args := [] },
+  { result := "range",  op := .make_range none,         args := [] },
   { result := "offset", op := .addi,              args := ["bstart", "range"] },
   { result := "aptrs",  op := .addptr,            args := ["a_base", "offset"] },
   { result := "bptrs",  op := .addptr,            args := ["b_base", "offset"] },
